src/examples/simple.v
@@ -89,15 +89,15 @@ Section simple_increment.
   (*
   Lemma wp_incr ℓa ℓb n E (Φ : val → dProp Σ) :
     ⊢ ℓa ↦ []; [0] | (λ s v, ⌜v = #s⌝) -∗
-      ℓb ↦ []; [0] | (λ s v, ⌜v = #s⌝ ∗ know_flush_lower_bound ℓa s) -∗
+      ℓb ↦ []; [0] | (λ s v, ⌜v = #s⌝ ∗ know_flush_lb ℓa s) -∗
       WPC (incr ℓa ℓb) @ n; E
         {{ λ _,
            ℓa ↦ []; [0; 1] | (λ s v, ⌜v = #s⌝) ∗ (* FIXME: The [0] should be moved left. *)
-           ℓb ↦ []; [0; 1] | (λ s v, ⌜v = #s⌝ ∗ know_flush_lower_bound ℓa s)
+           ℓb ↦ []; [0; 1] | (λ s v, ⌜v = #s⌝ ∗ know_flush_lb ℓa s)
         }}
         {{ ∃ (sa1 sa2 sb1 sb2 : list nat),
            ℓa ↦ sa1; sa2 | (λ s v, ⌜v = #s⌝) ∗
-           ℓb ↦ sb1; sb2 | (λ s v, ⌜v = #s⌝ ∗ know_flush_lower_bound ℓa s) }}.
+           ℓb ↦ sb1; sb2 | (λ s v, ⌜v = #s⌝ ∗ know_flush_lb ℓa s) }}.
   Proof.
     iIntros "aPts bPts".
     rewrite /incr.
